viper-total-heaps/TotalResult.thy
@@ -1,0 +1,61 @@
+theory TotalResult
+  imports ViperCommon.ViperLang ViperCommon.ValueAndBasicState TotalViperState ViperCommon.Binop ViperCommon.DeBruijn ViperCommon.PredicatesUtil TotalStateUtil
+begin
+
+datatype 'a result_total = RMagic | RFailure | RNormal "'a full_total_state"
+
+fun map_result_total :: "('a full_total_state \<Rightarrow> 'b full_total_state) \<Rightarrow> 'a result_total \<Rightarrow> 'b result_total"
+  where
+    "map_result_total f (RNormal \<omega>) = (RNormal (f \<omega>))"
+  | "map_result_total f RMagic = RMagic"
+  | "map_result_total f RFailure = RFailure"
+
+inductive th_result_rel :: "bool \<Rightarrow> bool \<Rightarrow> ('a full_total_state) set \<Rightarrow> 'a result_total \<Rightarrow> bool"  where
+  THResultNormal: "\<lbrakk> \<omega> \<in> W \<rbrakk> \<Longrightarrow> th_result_rel True True W (RNormal \<omega>)"
+| THResultMagic: "th_result_rel True False W RMagic"
+| THResultFailure: "th_result_rel False b W RFailure"
+
+text \<open>\<^const>\<open>th_result_rel\<close> is an auxiliary relation that is useful to express a state in terms of
+conditions. \<^term>\<open>th_result_rel bSuccess bFeasible W res\<close> is used in the following way:
+
+  \<^item> \<^term>\<open>bSuccess\<close> expresses when \<^term>\<open>res\<close> is not a failing state
+  \<^item> If \<^term>\<open>bSuccess\<close> holds (i.e., \<^term>\<open>res\<close> not a failing state), then
+    \<^term>\<open>bFeasible\<close> expresses when res is a normal state.
+  \<^item> W expresses the set of possible normal states for \<^term>\<open>res\<close> if both \<^term>\<open>bSuccess\<close> and
+    \<^term>\<open>bFeasible\<close> hold.
+\<close>
+
+inductive_cases THResultNormal_case: "th_result_rel True True W (RNormal \<omega>)"
+thm THResultNormal_case
+
+lemma THResultNormal_alt: "\<lbrakk> \<omega> \<in> W; A; B\<rbrakk> \<Longrightarrow> th_result_rel A B W (RNormal \<omega>)"
+  by (cases A; cases B) (auto intro: THResultNormal)
+
+lemma th_result_rel_normal:
+  assumes "th_result_rel a b W (RNormal \<omega>)"
+  shows "a \<and> b \<and> \<omega> \<in> W"
+  using assms
+  by (cases) auto
+
+text \<open>\<^typ>\<open>'a result_total\<close> expresses the possible states for statements. \<close>
+
+
+lemma th_result_rel_failure:
+  assumes "th_result_rel False b W res"
+  shows "res = RFailure"
+  using assms
+  by (cases) auto
+
+lemma th_result_rel_failure_2:
+  assumes "th_result_rel a b W RFailure"
+  shows "\<not>a"
+  using assms
+  by (cases) auto
+
+lemma th_result_rel_magic:
+  assumes "th_result_rel True False W res"
+  shows "res = RMagic"
+  using assms
+  by (cases) auto
+
+end
