viper-total-heaps/TotalSemanticsCoreHelper.thy
@@ -1,0 +1,262 @@
+theory TotalSemanticsCoreHelper
+  imports TotalSemanticsCore
+begin
+
+subsection \<open>Elimination and introduction rules\<close>
+
+(* lemmas red_exp_inhale_unfold_intros = red_pure_exp_total_red_pure_exps_total_red_inhale_unfold_rel.intros *)
+
+lemmas red_exp_intros = red_pure_exp_total_red_pure_exps_total.intros
+
+subsubsection \<open>Expression evaluation and well-definedness\<close>
+
+lemma RedField_no_def_normalI:
+  assumes "ctxt, None \<turnstile> \<langle>e; \<omega>\<rangle> [\<Down>]\<^sub>t Val (VRef (Address a))"
+      and "get_hh_total_full \<omega> (a, f) = v"
+    shows "ctxt, None \<turnstile> \<langle>FieldAcc e f; \<omega>\<rangle> [\<Down>]\<^sub>t Val v"
+proof -
+  let ?res = "(if (if_Some (\<lambda>res. (a,f) \<in> get_valid_locs res) (None :: ('a full_total_state) option)) then Val v else VFailure)"
+
+  have "ctxt, None \<turnstile> \<langle>FieldAcc e f; \<omega>\<rangle> [\<Down>]\<^sub>t ?res"
+    apply (rule RedField)
+    using assms
+    by auto
+
+  thus ?thesis
+    by simp
+qed
+
+lemma RedField_def_normalI:
+  assumes "ctxt, Some \<omega>_def \<turnstile> \<langle>e; \<omega>\<rangle> [\<Down>]\<^sub>t Val (VRef (Address a))"
+      and "get_hh_total_full \<omega> (a, f) = v"
+      and "(a,f) \<in> get_valid_locs \<omega>_def"
+    shows "ctxt, Some \<omega>_def \<turnstile> \<langle>FieldAcc e f; \<omega>\<rangle> [\<Down>]\<^sub>t Val v"
+proof -
+  let ?res = "(if (if_Some (\<lambda>res. (a,f) \<in> get_valid_locs res) (Some \<omega>_def)) then Val v else VFailure)"
+
+  have "ctxt, Some \<omega>_def \<turnstile> \<langle>FieldAcc e f; \<omega>\<rangle> [\<Down>]\<^sub>t ?res"
+    apply (rule RedField)
+    using assms
+    by auto
+
+  thus ?thesis
+    using assms
+    by simp
+qed
+
+lemma RedField_def_failureI:
+  assumes "ctxt, Some \<omega>_def \<turnstile> \<langle>e; \<omega>\<rangle> [\<Down>]\<^sub>t Val (VRef (Address a))"
+      and "get_hh_total_full \<omega> (a, f) = v"
+      and "(a,f) \<notin> get_valid_locs \<omega>_def"
+    shows "ctxt, Some \<omega>_def \<turnstile> \<langle>FieldAcc e f; \<omega>\<rangle> [\<Down>]\<^sub>t VFailure"
+proof -
+  let ?res = "(if (if_Some (\<lambda>res. (a,f) \<in> get_valid_locs res) (Some \<omega>_def)) then Val v else VFailure)"
+
+  have "ctxt, Some \<omega>_def \<turnstile> \<langle>FieldAcc e f; \<omega>\<rangle> [\<Down>]\<^sub>t ?res"
+    apply (rule RedField)
+    using assms
+    by auto
+
+  thus ?thesis
+    using assms
+    by simp
+qed
+
+inductive_cases RedVar_case: "ctxt, \<omega>_def \<turnstile> \<langle>Var n; \<omega>\<rangle> [\<Down>]\<^sub>t Val v"
+
+lemma RedLit_case:
+  assumes
+    "ctxt, \<omega>_def \<turnstile> \<langle>ELit l; \<omega>\<rangle> [\<Down>]\<^sub>t v" and
+    "v = Val (val_of_lit l) \<Longrightarrow> P"
+  shows P
+  using assms
+  by (cases) auto
+
+lemma RedFieldNormal_case:
+  assumes "ctxt, \<omega>_def \<turnstile> \<langle>FieldAcc e f; \<omega>\<rangle> [\<Down>]\<^sub>t Val v" and
+          "\<And>a. ctxt, \<omega>_def \<turnstile> \<langle>e;\<omega>\<rangle> [\<Down>]\<^sub>t Val (VRef (Address a)) \<Longrightarrow>
+           (if_Some (\<lambda>res. (a,f) \<in> get_valid_locs res) \<omega>_def) \<Longrightarrow>
+           get_hh_total_full \<omega> (a, f) = v \<Longrightarrow>
+             P"
+        shows P
+  using assms
+  by cases (metis extended_val.distinct(1) extended_val.inject)
+
+inductive_cases RedUnop_case: "ctxt, \<omega>_def \<turnstile> \<langle>Unop unop e; \<omega>\<rangle> [\<Down>]\<^sub>t Val v'"
+inductive_cases RedBinop_case: "ctxt, \<omega>_def \<turnstile> \<langle>Binop e1 bop e2; \<omega>\<rangle> [\<Down>]\<^sub>t Val v"
+inductive_cases RedFunApp_case: "ctxt, \<omega>_def \<turnstile> \<langle>FunApp fname es; \<omega>\<rangle> [\<Down>]\<^sub>t res"
+
+inductive_cases RedExpList_case: "red_pure_exps_total ctxt LH es \<omega> (Some vs)"
+inductive_cases RedExpListFailure_case: "red_pure_exps_total ctxt LH es \<omega> None"
+inductive_cases RedExpListGeneral_case: "red_pure_exps_total ctxt LH es \<omega> res"
+
+lemma red_exp_list_normal_elim:
+  assumes
+     "red_pure_exps_total ctxt \<omega>_def es \<omega> (Some vs)" and
+     "(\<And>vs_hd vs_tl e_hd es_tl.
+        es = e_hd # es_tl \<Longrightarrow>
+        vs = vs_hd # vs_tl \<Longrightarrow>
+        ctxt, \<omega>_def \<turnstile> \<langle>e_hd;\<omega>\<rangle> [\<Down>]\<^sub>t Val vs_hd \<Longrightarrow> red_pure_exps_total ctxt \<omega>_def es_tl \<omega> (Some vs_tl) \<Longrightarrow> P)" and
+     "es = [] \<Longrightarrow> vs = [] \<Longrightarrow> P"
+   shows "P"
+  using assms
+proof cases
+  case (RedExpListCons e v es' res)
+  from this obtain vs' where "res = Some vs'" and "vs = v#vs'"
+    by (metis map_option_eq_Some)
+  with RedExpListCons assms(2)[OF \<open>es = e#es'\<close> \<open>vs = _\<close> ]  show ?thesis
+    by blast
+next
+  case RedExpListNil
+  then show ?thesis using assms by auto
+qed
+
+lemma red_exp_list_failure_Nil:
+  assumes "red_pure_exps_total ctxt_vpr \<omega>_def [] \<omega> res"
+  shows "res = Some []"
+  using assms
+  by cases
+
+lemma red_exp_list_failure_elim:
+  assumes
+     "red_pure_exps_total ctxt \<omega>_def es \<omega> None" and
+     "(\<And>v e_hd es_tl.
+        es = e_hd # es_tl \<Longrightarrow>
+        ctxt, \<omega>_def \<turnstile> \<langle>e_hd;\<omega>\<rangle> [\<Down>]\<^sub>t (Val v) \<Longrightarrow>
+        es_tl \<noteq> [] \<Longrightarrow>
+        red_pure_exps_total ctxt \<omega>_def es_tl \<omega> None \<Longrightarrow> P)" and
+     "(\<And>e_hd es_tl.
+        es = e_hd # es_tl \<Longrightarrow>
+        ctxt, \<omega>_def \<turnstile> \<langle>e_hd;\<omega>\<rangle> [\<Down>]\<^sub>t VFailure \<Longrightarrow> P)"
+   shows "P"
+  using assms
+  by (cases) (auto elim: RedExpListFailure_case)
+
+lemma red_exp_list_failure_nth:
+  assumes "red_pure_exps_total ctxt \<omega>_def es \<omega> None" and
+          "es \<noteq> []"
+  shows "\<exists>i. i < length es \<and> ctxt, \<omega>_def \<turnstile> \<langle>es ! i;\<omega>\<rangle> [\<Down>]\<^sub>t VFailure"
+  using assms
+proof (induction es)
+  case Nil
+  then show ?case by simp \<comment>\<open>contradiction\<close>
+next
+  case (Cons a es)
+  thus ?case
+    by (fastforce elim: red_exp_list_failure_elim dest!: Cons.IH)
+qed
+
+inductive_cases RedPerm_case: "ctxt, \<omega>_def \<turnstile> \<langle>Perm e f; \<omega>\<rangle> [\<Down>]\<^sub>t Val v"
+
+lemma red_pure_exps_total_singleton:
+  assumes "red_pure_exps_total ctxt \<omega>_def [e] \<omega> res" and
+          "\<And>v. res = Some [v] \<and> (ctxt, \<omega>_def \<turnstile> \<langle>e; \<omega>\<rangle> [\<Down>]\<^sub>t Val v) \<Longrightarrow> P" and
+          "res = None \<Longrightarrow> ctxt, \<omega>_def \<turnstile> \<langle>e; \<omega>\<rangle> [\<Down>]\<^sub>t VFailure \<Longrightarrow> P"
+  shows P
+  apply (rule RedExpListGeneral_case[OF assms(1)])
+  using RedExpListGeneral_case assms(2) apply blast
+   apply (simp add: assms(3))
+  apply simp
+  done
+
+lemmas red_pure_exp_total_elims =
+  RedLit_case RedVar_case
+  RedUnop_case RedBinop_case RedFunApp_case
+  red_exp_list_normal_elim red_exp_list_failure_elim
+
+lemma red_pure_exps_total_append_failure:
+  assumes "red_pure_exps_total ctxt \<omega>_def es \<omega> None"
+  shows "red_pure_exps_total ctxt \<omega>_def (es@es') \<omega> None"
+  using assms
+proof (induction es)
+  case Nil
+  then show ?case
+    using red_exp_list_failure_Nil
+    by blast
+next
+  case (Cons e es)
+  then show ?case
+    by (auto elim: red_exp_list_failure_elim intro: red_exp_intros)
+qed
+
+lemma red_pure_exps_total_append_failure_2:
+  assumes "red_pure_exps_total ctxt \<omega>_def es \<omega> (Some vs)"
+      and "red_pure_exps_total ctxt \<omega>_def es' \<omega> None"
+    shows "red_pure_exps_total ctxt \<omega>_def (es@es') \<omega> None"
+  using assms
+proof (induction es arbitrary: vs)
+  case Nil
+  then show ?case by simp
+next
+  case (Cons e es)
+  from this obtain v vs_tl where
+     "vs = v#vs_tl" and
+     RedE: "ctxt, \<omega>_def \<turnstile> \<langle>e; \<omega>\<rangle> [\<Down>]\<^sub>t Val v"
+     "red_pure_exps_total ctxt \<omega>_def es \<omega> (Some vs_tl)"
+  by (auto elim: red_pure_exp_total_elims)
+
+  then have "red_pure_exps_total ctxt \<omega>_def (es @ es') \<omega> None"
+    using Cons
+    by blast
+
+  thus ?case
+    using RedE
+    by (auto intro: red_exp_intros)
+qed
+
+subsubsection \<open>Inhale\<close>
+
+lemma inh_imp_failure:
+  assumes "ctxt, Some \<omega> \<turnstile> \<langle>e;\<omega>\<rangle> [\<Down>]\<^sub>t VFailure"
+  shows "red_inhale ctxt (Imp e A) \<omega> RFailure"
+  using assms InhSubExpFailure[where ?A="Imp e A"] RedExpListFailure
+  by fastforce
+
+lemma inh_cond_assert_failure:
+  assumes "ctxt, Some \<omega> \<turnstile> \<langle>e;\<omega>\<rangle> [\<Down>]\<^sub>t VFailure"
+  shows "red_inhale ctxt (CondAssert e A B) \<omega> RFailure"
+  using assms InhSubExpFailure[where ?A="CondAssert e A B"] RedExpListFailure
+  by fastforce
+
+lemma inh_pure_normal:
+  assumes "ctxt, Some \<omega> \<turnstile> \<langle>e;\<omega>\<rangle> [\<Down>]\<^sub>t Val (VBool True)"
+  shows "red_inhale ctxt (Atomic (Pure e)) \<omega> (RNormal \<omega>)"
+  using assms InhPure
+  by force
+
+lemma inh_pure_magic:
+  assumes "ctxt, Some \<omega> \<turnstile> \<langle>e;\<omega>\<rangle> [\<Down>]\<^sub>t Val (VBool False)"
+  shows "red_inhale ctxt (Atomic (Pure e)) \<omega> RMagic"
+  using assms InhPure
+  by force
+
+lemmas red_inhale_intros =
+  InhAcc
+  InhAccPred
+  InhAccWildcard
+  InhAccPredWildcard
+  inh_pure_normal
+  inh_pure_magic
+  InhStarNormal
+  InhStarFailureMagic
+  InhImpTrue
+  InhImpFalse
+  InhCondAssertTrue
+  InhCondAssertFalse
+  InhSubExpFailure
+
+inductive_cases InhStar_case: "red_inhale ctxt (A && B) \<omega> res"
+inductive_cases InhImp_case: "red_inhale ctxt (Imp e A) \<omega> res"
+inductive_cases InhPure_case: "red_inhale ctxt (Atomic (Pure e)) \<omega> res"
+thm InhPure_case
+
+lemmas red_inhale_elims =
+  InhStar_case
+  InhImp_case
+  InhPure_case
+
+subsubsection \<open>Unfold\<close>
+
+(* inductive_cases UnfoldRel_case: "unfold_rel ctxt pred_id vs q \<phi> \<phi>'" *)
+
+end
